experiment/Experiment.Steel.Repr.LV_to_M.fsti
@@ -50,17 +50,66 @@ val extract_eij_framed_equiv
                        (filter_sl (mask_not (eij_trg_mask csm_f)) sl))
 
 
+let spec_post_equiv
+      (env : vprop_list)
+      (pre post ro : vprop_list)
+      (pre_f : eq_injection_l L.(pre @ ro) env)
+  : vequiv_perm L.((post @ ro) @ filter_mask (mask_not (eij_trg_mask pre_f)) env)
+                  (res_env env (eij_trg_mask (eij_split pre ro pre_f)._1) post)
+  =
+    let m_trg  = eij_trg_mask pre_f                 in
+    let csm_f  = (eij_split pre ro pre_f)._1        in
+    let m_trg0 = eij_trg_mask csm_f                 in
+    let env1   = filter_mask (mask_not m_trg0) env  in
+    let ro_f1  : eq_injection_l ro env1
+               = eij_split1 pre ro pre_f            in
+    let m_trg1 = eij_trg_mask ro_f1                 in
+    let flt0   = filter_mask m_trg1 env1            in
+    let flt1   = filter_mask (mask_not m_trg1) env1 in
+    L.(calc (==) {
+      (post @ ro) @ filter_mask (mask_not m_trg) env;
+    == { append_assoc post ro (filter_mask (mask_not m_trg) env) }
+      post @ ro @ filter_mask (mask_not m_trg) env;
+    == { eij_split1_trg_mask pre ro pre_f }
+      post @ ro @ filter_mask (mask_not (mask_comp_or m_trg0 m_trg1)) env;
+    == { mask_not_comp_or m_trg0 m_trg1;
+         filter_mask_and (mask_not m_trg0) (mask_not m_trg1) env }
+      post @ (ro @ flt1);
+    });
+    assert L.(res_env env (eij_trg_mask (eij_split pre ro pre_f)._1) post == post @ env1);
+    
+    let f0 : vequiv_perm ro flt0
+      = Perm.pequiv_sym (eij_equiv ro_f1)  in
+    let f1 : vequiv_perm L.(flt0 @ flt1) env1
+      = mask_pequiv_append' m_trg1 env1    in
+    let f2 : vequiv_perm L.(post @ (ro @ flt1)) L.(post @ env1)
+      = Perm.pequiv_append (Perm.pequiv_refl post)
+          (Perm.pequiv_trans
+            (Perm.pequiv_append f0 (Perm.pequiv_refl flt1))
+            f1)
+    in
+    U.cast _ f2
+
+val extract_spec_post_equiv
+      (env : vprop_list) (pre post ro : vprop_list) (pre_f : eq_injection_l L.(pre @ ro) env)
+      (sl0 : sl_f env) (sl_post : sl_f post)
+  : Lemma (extract_vars (spec_post_equiv env pre post ro pre_f)
+                        (append_vars (append_vars sl_post (split_vars pre ro (eij_sl (L.index pre_f) sl0))._2)
+                                     (filter_sl (mask_not (eij_trg_mask pre_f)) sl0))
+        == append_vars sl_post (filter_sl (mask_not (eij_trg_mask (eij_split pre ro pre_f)._1)) sl0))
+
+
 let repr_M_of_LV__tcs
       (env : vprop_list)
-      (a : Type u#a) (pre : M.pre_t) (post : M.post_t a)
-      (csm_f : eq_injection_l pre env)
-  : M.tree_cond_Spec a pre post
+      (a : Type u#a) (s : M.spec_r a)
+      (pre_f : eq_injection_l (M.spc_pre1 s) env)
+  : M.tree_cond_Spec a (M.spc_pre1 s) (M.spc_post1 s)
   = {
     tcs_pre     = env;
-    tcs_post    = res_env_f env (eij_trg_mask csm_f) post;
-    tcs_frame   = filter_mask (mask_not (eij_trg_mask csm_f)) env;
-    tcs_pre_eq  = Veq.vequiv_of_perm (eij_framed_equiv env pre csm_f);
-    tcs_post_eq = (fun x -> Veq.vequiv_refl L.(post x @ filter_mask (mask_not (eij_trg_mask csm_f)) env))
+    tcs_post    = res_env_f env (spec_csm pre_f) s.spc_post;
+    tcs_frame   = filter_mask (mask_not (eij_trg_mask pre_f)) env;
+    tcs_pre_eq  = Veq.vequiv_of_perm (eij_framed_equiv env (M.spc_pre1 s) pre_f);
+    tcs_post_eq = (fun x -> Veq.vequiv_of_perm (spec_post_equiv env s.spc_pre (s.spc_post x) s.spc_ro pre_f));
   }
 
 #push-options "--ifuel 0 --fuel 0"
@@ -107,22 +156,30 @@ val extract_sub_prd_framed_equiv
     == append_vars (extract_vars veq (append_vars sl0 (filter_sl csm1 sl1)))
                    (filter_sl (mask_not csm1) sl1))
 
+let spec_sub_post_equiv
+      (env : vprop_list) (#a : Type) (s : M.spec_r a) (pre_f : eq_injection_l (M.spc_pre1 s) env)
+      (csm1 : csm_t (filter_mask (mask_not (spec_csm pre_f)) env)) (prd1 : prd_t a)
+      (prd_f1 : (x : a) -> Perm.pequiv_list (sub_prd env (spec_csm pre_f) (s.spc_post x) csm1) (prd1 x))
+      (x : a)
+  : vequiv_perm L.(M.spc_post1 s x @ filter_mask (mask_not (eij_trg_mask pre_f)) env)
+                  (res_env env (bind_csm env (spec_csm pre_f) csm1) (prd1 x))
+  = Perm.pequiv_trans (spec_post_equiv env s.spc_pre (s.spc_post x) s.spc_ro pre_f)
+                      (sub_prd_framed_equiv env (spec_csm pre_f) (s.spc_post x)
+                                            csm1 (prd1 x) (Perm.perm_f_of_list (prd_f1 x)))
 
 let repr_M_of_LV__tcs_sub
       (env : vprop_list)
-      (a : Type u#a) (pre : M.pre_t) (post : M.post_t a)
-      (csm_f : eq_injection_l pre env)
-      (csm1 : csm_t (filter_mask (mask_not (eij_trg_mask csm_f)) env)) (prd1 : prd_t a)
-      (prd_f1 : (x : a) -> Perm.pequiv_list (sub_prd env (eij_trg_mask csm_f) (post x) csm1) (prd1 x))
-  : M.tree_cond_Spec a pre post
+      (a : Type u#a) (s : M.spec_r a)
+      (pre_f : eq_injection_l (M.spc_pre1 s) env)
+      (csm1 : csm_t (filter_mask (mask_not (spec_csm pre_f)) env)) (prd1 : prd_t a)
+      (prd_f1 : (x : a) -> Perm.pequiv_list (sub_prd env (spec_csm pre_f) (s.spc_post x) csm1) (prd1 x))
+  : M.tree_cond_Spec a (M.spc_pre1 s) (M.spc_post1 s)
   = {
     tcs_pre     = env;
-    tcs_post    = res_env_f env (bind_csm env (eij_trg_mask csm_f) csm1) prd1;
-    tcs_frame   = filter_mask (mask_not (eij_trg_mask csm_f)) env;
-    tcs_pre_eq  = Veq.vequiv_of_perm (eij_framed_equiv env pre csm_f);
-    tcs_post_eq = (fun x -> Veq.vequiv_of_perm (
-                           sub_prd_framed_equiv env (eij_trg_mask csm_f) (post x)
-                               csm1 (prd1 x) (Perm.perm_f_of_list (prd_f1 x))))
+    tcs_post    = res_env_f env (bind_csm env (spec_csm pre_f) csm1) prd1;
+    tcs_frame   = filter_mask (mask_not (eij_trg_mask pre_f)) env;
+    tcs_pre_eq  = Veq.vequiv_of_perm (eij_framed_equiv env (M.spc_pre1 s) pre_f);
+    tcs_post_eq = (fun x -> Veq.vequiv_of_perm (spec_sub_post_equiv env s pre_f csm1 prd1 prd_f1 x))
   }
 
 val bind_g_csm'_res_env_f
@@ -142,8 +199,8 @@ let rec repr_M_of_LV
       (lc : lin_cond env t csm prd)
   : Pure (lc_to_M lc) (requires lcsub_at_leaves lc) (ensures fun _ -> True) (decreases lc)
   = match lc with
-  | LCspec env #a #sp s sh csm_f ->
-      M.TCspec #a #sp s sh  (repr_M_of_LV__tcs env a s.spc_pre s.spc_post csm_f)
+  | LCspec env #a #sp s sh pre_f ->
+      M.TCspec #a #sp s sh  (repr_M_of_LV__tcs env a s pre_f)
   | LCret env #a #x #sl_hint prd csm_f ->
       M.TCret #a #x #sl_hint
           env (fun x' -> L.(prd x' @ filter_mask (mask_not (eij_trg_mask csm_f)) env))
@@ -161,11 +218,11 @@ let rec repr_M_of_LV
           (repr_M_of_LV cthn)
           (repr_M_of_LV cels)
   | LCsub env #a0 #f0 csm0 prd0 cf csm1 prd1 prd_f1 ->
-      let LCspec env #a #sp s sh csm_f = cf in
-      let prd_f1 (x : a) : Perm.pequiv_list (sub_prd env (eij_trg_mask csm_f) (s.spc_post x) csm1) (prd1 x)
+      let LCspec env #a #sp s sh pre_f = cf in
+      let prd_f1 (x : a) : Perm.pequiv_list (sub_prd env (spec_csm pre_f) (s.spc_post x) csm1) (prd1 x)
             = U.cast _ (prd_f1 x)
       in
-      M.TCspec #a #sp s sh (repr_M_of_LV__tcs_sub env a s.spc_pre s.spc_post csm_f csm1 prd1 prd_f1)
+      M.TCspec #a #sp s sh (repr_M_of_LV__tcs_sub env a s pre_f csm1 prd1 prd_f1)
 #pop-options
 
 #push-options "--ifuel 0 --fuel 0"
